Changed make_full_observation to defer outputs like SAL does

theories/efsm-ltl/EFSM_LTL.thy
@@ -37,14 +37,21 @@ lemma ltl_step_alt:  "ltl_step e (Some s) r t = (let possibilities = possible_st
 lemma ltl_step_none: "possible_steps e s r (fst ie) (snd ie) = {||} \<Longrightarrow> ltl_step e (Some s) r ie = (None, [], r)"
   by (simp add: ltl_step_alt)
 
-primcorec make_full_observation :: "transition_matrix \<Rightarrow> nat option \<Rightarrow> registers \<Rightarrow> event stream \<Rightarrow> state stream" where
-  "make_full_observation e s d i = (let (s', o', d') = ltl_step e s d (shd i) in \<lparr>statename = s, datastate = d, event=(shd i), output = o'\<rparr>##(make_full_observation e s' d' (stl i)))"
+primcorec make_full_observation :: "transition_matrix \<Rightarrow> nat option \<Rightarrow> registers \<Rightarrow> outputs \<Rightarrow> event stream \<Rightarrow> state stream" where
+  "make_full_observation e s d p i = (
+    let (s', o', d') = ltl_step e s d (shd i) in
+    \<lparr>statename = s, datastate = d, event=(shd i), output = p\<rparr>##(make_full_observation e s' d' o' (stl i))
+  )"
 
 definition watch :: "transition_matrix \<Rightarrow> event stream \<Rightarrow> state stream" where
-  "watch e i \<equiv> (make_full_observation e (Some 0) <> i)"
+  "watch e i \<equiv> (make_full_observation e (Some 0) <> [] i)"
 
 definition state_eq :: "nat option \<Rightarrow> state stream \<Rightarrow> bool" where
   "state_eq v s \<equiv> statename (shd s) = v"
+
+lemma state_eq_holds: "state_eq s = holds (\<lambda>x. statename x = s)"
+  apply (rule ext)
+  by (simp add: state_eq_def holds_def)
 
 lemma state_eq_None_not_Some: "state_eq None s \<Longrightarrow> \<not> state_eq (Some n) s"
   by (simp add: state_eq_def)
@@ -64,22 +71,24 @@ definition event_eq :: "(string \<times> inputs) \<Rightarrow> state stream \<Ri
 definition output_eq :: "value option list \<Rightarrow> state stream \<Rightarrow> bool" where
   "output_eq v s \<equiv> output (shd s) = v"
 
-lemma shd_state_is_none: "(state_eq None) (make_full_observation e None r t)"
+lemma shd_state_is_none: "(state_eq None) (make_full_observation e None r p t)"
   by (simp add: state_eq_def)
 
-lemma unfold_observe_none: "make_full_observation e None d t = (\<lparr>statename = None, datastate = d, event=(shd t), output = []\<rparr>##(make_full_observation e None d (stl t)))"
+lemma unfold_observe_none: "make_full_observation e None d p t = (\<lparr>statename = None, datastate = d, event=(shd t), output = p\<rparr>##(make_full_observation e None d [] (stl t)))"
   by (simp add: stream.expand)
 
-lemma once_none_always_none: "alw (state_eq None) (make_full_observation e None r t)"
+lemma once_none_always_none: "alw (state_eq None) (make_full_observation e None r p t)"
 proof -
-  obtain ss :: "((String.literal \<times> value list) stream \<Rightarrow> state stream) \<Rightarrow> (String.literal \<times> value list) stream" where
-    "\<forall>f p s. f (stl (ss f)) \<noteq> stl (f (ss f)) \<or> alw p (f s) = alw (\<lambda>s. p (f s)) s"
+  obtain ssa :: "((String.literal \<times> value list) stream \<Rightarrow> state stream) \<Rightarrow> (String.literal \<times> value list) stream" where
+      "\<forall>f p s. f (stl (ssa f)) \<noteq> stl (f (ssa f)) \<or> alw p (f s) = alw (\<lambda>s. p (f s)) s"
     by (metis (no_types) alw_inv)
+  then have "alw (state_eq None) (make_full_observation e None r [] (stl t))"
+    by (metis (no_types) all_imp_alw shd_state_is_none stream.sel(2) unfold_observe_none)
   then show ?thesis
-    by (simp add: state_eq_def all_imp_alw)
+    by (metis (no_types) alw.simps shd_state_is_none stream.sel(2) unfold_observe_none)
 qed
 
-lemma no_output_none: "alw (output_eq []) (make_full_observation e None r t)"
+lemma no_output_none: "nxt (alw (output_eq [])) (make_full_observation e None r p t)"
 proof -
   obtain ss :: "((String.literal \<times> value list) stream \<Rightarrow> state stream) \<Rightarrow> (String.literal \<times> value list) stream" where
     "\<forall>f p s. f (stl (ss f)) \<noteq> stl (f (ss f)) \<or> alw p (f s) = alw (\<lambda>s. p (f s)) s"
@@ -88,28 +97,47 @@ proof -
     by (simp add: output_eq_def all_imp_alw)
 qed
 
-lemma no_updates_none: "alw (\<lambda>x. datastate (shd x) = r) (make_full_observation e None r t)"
+lemma no_output_none_nxt: "alw (nxt (output_eq [])) (make_full_observation e None r p t)"
+  by (metis alw_inv alw_mono no_output_none nxt.simps)
+
+lemma no_updates_none: "alw (\<lambda>x. datastate (shd x) = r) (make_full_observation e None r p t)"
 proof -
-  obtain ss :: "((String.literal \<times> value list) stream \<Rightarrow> state stream) \<Rightarrow> (String.literal \<times> value list) stream" where
-    "\<forall>f p s. f (stl (ss f)) \<noteq> stl (f (ss f)) \<or> alw p (f s) = alw (\<lambda>s. p (f s)) s"
-    by (metis (no_types) alw_inv)
-  then show ?thesis
-    by (simp add: all_imp_alw)
+  have "alw (\<lambda>x. datastate (shd x) = r) (make_full_observation e None r [] (stl t))"
+    proof -
+      obtain ss :: "((String.literal \<times> value list) stream \<Rightarrow> state stream) \<Rightarrow> (String.literal \<times> value list) stream" where
+        "\<forall>f p s. f (stl (ss f)) \<noteq> stl (f (ss f)) \<or> alw p (f s) = alw (\<lambda>s. p (f s)) s"
+        by (metis (no_types) alw_inv)
+      then show ?thesis
+        by (simp add: output_eq_def all_imp_alw)
+    qed
+    then show ?thesis
+    proof(coinduction)
+      case alw
+      then show ?case
+        by simp
+    qed
 qed
 
 lemma event_components: "(label_eq l aand input_eq i) s = (event (shd s) = (String.implode l, i))"
   apply (simp add: label_eq_def input_eq_def)
   by (metis fst_conv prod.collapse snd_conv)
 
-lemma alw_not_some: "alw (\<lambda>xs. statename (shd xs) \<noteq> Some s) (make_full_observation e None r t)"
-  using once_none_always_none[of e r t]
-  unfolding state_eq_def
-  by (simp add: alw_mono)
+lemma alw_not_some: "alw (\<lambda>xs. statename (shd xs) \<noteq> Some s) (make_full_observation e None r p t)"
+  by (metis (mono_tags, lifting) alw_mono once_none_always_none option.distinct(1) state_eq_def)
+
+lemma state_none: "((state_eq None) impl nxt (state_eq None)) (make_full_observation e s r p t)"
+  by (simp add: state_eq_def)
+
+lemma state_none_2: "(state_eq None) (make_full_observation e s r p t) \<Longrightarrow> (state_eq None) (make_full_observation e s r p (stl t))"
+  by (simp add: state_eq_def)
 
 lemma decompose_pair: "e \<noteq> (l, i) = (\<not> (fst e =l \<and> snd e = i))"
   by (metis fst_conv prod.collapse sndI)
 
 definition check_exp :: "ltl_gexp \<Rightarrow> state stream \<Rightarrow> bool" where
   "check_exp g s = (gval g (snd (event (shd s))) (datastate (shd s)) (output (shd s)) = trilean.true)"
+
+lemma alw_ev: "alw f = not (ev (\<lambda>s. \<not>f s))"
+  by simp
 
 end
